more porting

Weidenbach_Book/IsaSAT/IsaSAT_Bump_Heuristics_State.thy
@@ -1,11 +1,13 @@
 theory IsaSAT_Bump_Heuristics_State
-imports Watched_Literals_VMTF
+imports Watched_Literals_VMTF 
+(*
   IsaSAT_VSIDS
+  *)
   Tuple4
 begin
 
 (*TODO: share the to_remove part of Bump_Heuristics*)
-type_synonym bump_heuristics = \<open>(vmtf_remove_int, vmtf_remove_int, bool, nat) tuple4\<close>
+type_synonym bump_heuristics = \<open>(vmtf, vmtf, bool, nat list \<times> bool list) tuple4\<close>
 
 abbreviation Bump_Heuristics :: \<open>_ \<Rightarrow> _ \<Rightarrow> _ \<Rightarrow> _ \<Rightarrow> bump_heuristics\<close> where
   \<open>Bump_Heuristics a b c d \<equiv> Tuple4 a b c d\<close>
@@ -13,29 +15,29 @@ abbreviation Bump_Heuristics :: \<open>_ \<Rightarrow> _ \<Rightarrow> _ \<Right
 lemmas bump_heuristics_splits = Tuple4.tuple4.splits
 hide_fact tuple4.splits
 
-abbreviation get_stable_heuristics :: \<open>bump_heuristics \<Rightarrow> vmtf_remove_int\<close> where
+abbreviation get_stable_heuristics :: \<open>bump_heuristics \<Rightarrow> vmtf\<close> where
   \<open>get_stable_heuristics \<equiv> Tuple4_a\<close>
 
-abbreviation get_focused_heuristics :: \<open>bump_heuristics \<Rightarrow> vmtf_remove_int\<close> where
+abbreviation get_focused_heuristics :: \<open>bump_heuristics \<Rightarrow> vmtf\<close> where
   \<open>get_focused_heuristics \<equiv> Tuple4_b\<close>
 
 abbreviation is_focused_heuristics :: \<open>bump_heuristics \<Rightarrow> bool\<close> where
   \<open>is_focused_heuristics \<equiv> Tuple4_c\<close>
 
-abbreviation conflict_count :: \<open>bump_heuristics \<Rightarrow> nat\<close> where
-  \<open>conflict_count \<equiv> Tuple4_d\<close>
+abbreviation get_bumped_variables :: \<open>bump_heuristics \<Rightarrow> nat list \<times> bool list\<close> where
+  \<open>get_bumped_variables \<equiv> Tuple4_d\<close>
 
-abbreviation set_stable_heuristics :: \<open>vmtf_remove_int \<Rightarrow>bump_heuristics \<Rightarrow> _\<close> where
+abbreviation set_stable_heuristics :: \<open>vmtf \<Rightarrow>bump_heuristics \<Rightarrow> _\<close> where
   \<open>set_stable_heuristics \<equiv> Tuple4.set_a\<close>
 
-abbreviation set_focused_heuristics :: \<open>vmtf_remove_int \<Rightarrow>bump_heuristics \<Rightarrow> _\<close> where
+abbreviation set_focused_heuristics :: \<open>vmtf \<Rightarrow>bump_heuristics \<Rightarrow> _\<close> where
   \<open>set_focused_heuristics \<equiv> Tuple4.set_b\<close>
 
 abbreviation set_is_focused_heuristics :: \<open>bool \<Rightarrow>bump_heuristics \<Rightarrow> _\<close> where
   \<open>set_is_focused_heuristics \<equiv> Tuple4.set_c\<close>
 
-abbreviation set_conflict_count :: \<open>nat \<Rightarrow>bump_heuristics \<Rightarrow> _\<close> where
-  \<open>set_conflict_count \<equiv> Tuple4.set_d\<close>
+abbreviation set_bumped_variables :: \<open>nat list \<times> bool list \<Rightarrow>bump_heuristics \<Rightarrow> _\<close> where
+  \<open>set_bumped_variables \<equiv> Tuple4.set_d\<close>
 
 definition bump_heur :: \<open>_ \<Rightarrow> _ \<Rightarrow> bump_heuristics set\<close> where
   \<open>bump_heur \<A> M = {x.
@@ -44,7 +46,9 @@ definition bump_heur :: \<open>_ \<Rightarrow> _ \<Rightarrow> bump_heuristics s
       get_focused_heuristics x \<in> vmtf \<A> (takeWhile (\<lambda>x. \<not>is_decided x) M)) \<and>
     \<not>is_focused_heuristics x \<longrightarrow>
       (get_stable_heuristics x \<in> vmtf \<A> (takeWhile (\<lambda>x. \<not>is_decided x) M) \<and>
-      get_focused_heuristics x \<in> vmtf \<A> M)}\<close>
+       get_focused_heuristics x \<in> vmtf \<A> M) \<and>
+  (get_bumped_variables x, set (fst (get_bumped_variables x))) \<in> distinct_atoms_rel \<A>
+  }\<close>
 
 definition switch_bump_heur :: \<open>bump_heuristics \<Rightarrow> bump_heuristics\<close> where
   \<open>switch_bump_heur x = do {
@@ -80,11 +84,11 @@ lemma isa_vmtf_unset_vmtf_tl:
   shows \<open>isa_vmtf_unset L x \<in> bump_heur \<A> (tl M)\<close>
 proof -
   obtain ns m fst_As lst_As next_search remove where
-    \<open>is_focused_heuristics x \<Longrightarrow> get_focused_heuristics x = ((ns, m, fst_As, lst_As, next_search), remove)\<close>
-    \<open>\<not>is_focused_heuristics x \<Longrightarrow> get_stable_heuristics x = ((ns, m, fst_As, lst_As, next_search), remove)\<close>
+    \<open>is_focused_heuristics x \<Longrightarrow> get_focused_heuristics x = ((ns, m, fst_As, lst_As, next_search))\<close>
+    \<open>\<not>is_focused_heuristics x \<Longrightarrow> get_stable_heuristics x = ((ns, m, fst_As, lst_As, next_search))\<close>
    by (cases \<open>get_focused_heuristics x\<close>; cases \<open>get_stable_heuristics x\<close>; cases \<open>is_focused_heuristics x\<close>) auto
   show ?thesis
-    using vmtf_unset_vmtf_tl[of ns m fst_As lst_As next_search remove \<A> M]
+    using vmtf_unset_vmtf_tl[of ns m fst_As lst_As next_search \<A> M]
       assms by (auto simp: bump_heur_def)
 qed
 
