Weidenbach_Book/IsaSAT/IsaSAT_Simplify_Forward_Subsumption.thy
@@ -3812,7 +3812,7 @@ lemma get_conflict_wl_is_None_heur_get_conflict_wl_is_None_restart_occs:
   \<open>(RETURN o get_conflict_wl_is_None_heur,  RETURN o get_conflict_wl_is_None) \<in>
     twl_st_heur_restart_occs \<rightarrow>\<^sub>f \<langle>Id\<rangle>nres_rel\<close>
   unfolding get_conflict_wl_is_None_heur_def get_conflict_wl_is_None_def comp_def
-  apply (intro WB_More_Refinement.frefI nres_relI) apply refine_rcg
+  apply (intro frefI nres_relI) apply refine_rcg
   by (auto simp: twl_st_heur_restart_occs_def get_conflict_wl_is_None_heur_def get_conflict_wl_is_None_def
       option_lookup_clause_rel_def
      split: option.splits)
